It is trivial to show that the above is true of $ \mathcal E = 0 \lor \mathcal E = \mathcal L (V) $. The challenge is showing that it is false for any other $ \mathcal E $.

Call $ n = dim V $.

Make a list of length $ n^2 $ of $ n \times n $ matrices such that each is filled with zeroes, except for one non-zero entry in distinct slots. So, if $ n = 2 $, then 
$$ \begin{pmatrix}1 & 0\\\ 0 & 0\end{pmatrix} , \begin{pmatrix}0 & 1\\\ 0 & 0\end{pmatrix}, \begin{pmatrix}0 & 0\\\ 1 & 0\end{pmatrix},\begin{pmatrix}0 & 0\\\ 0 & 1\end{pmatrix} $$

This is obviously a basis of $ \mathcal L (V) $. 

Now, to consider a case where $ \mathcal E \neq \{0\} \land \mathcal E \neq \mathcal L(V) $, just remove at most $ n - 1 $ operators (vectors in $ \mathcal L(V) $'s basis) above. What results is the basis of a proper subspace of $ \mathcal L(V) $.

So now, you just have to find $ S \in \mathcal L(V), T \in \mathcal E $ such that the new basis cannot linearly combine into either $ ST $ or $ TS $.

If $ \mathcal E $'s basis is $ A_1, A_2, \cdots, A_m $, where $ 0 < m < n^2 $ then there must be at least one zero-entry shared across all vectors in the basis. Choose $ j,k $ such that for all vectors in the basis $ A_{j,k} = 0 $ and choose $ z, T $, where $ 0 < z < n $ and $ T \in A_1, \cdots, A_{n^2} $ such that there is at least one vector in the basis such that $ T_{z,k} \neq 0 \lor T_{j,z} \neq 0 $.

Consider that, for any compatible matrices $ A $ and $ B $, $ (AB)_{j,k} = \sum_{i=1}^{w} A_{j,i} B_{i,k} $. In the example above, if $ T_{z,k} \neq 0 $, there must be an $ S \in \mathcal L (V) $ such that $ (ST)_{j,k} = \sum_{i=1}^{n^2} S_{j,i} T_{i,k} $. For example, consider the matrix $ S $ where all entries are null except $ S_{j,z} $. In that case, $ (ST)_{j,k} = S_{j,i} T_{i,k} $, therefore it is non-zero, as $ \forall a,b \in F . (a b = 0) \to (a = 0) \lor (b = 0) $. Since such an entry in the product is nonzero, and the same entry is zero in all vectors of $ \mathcal E $'s basis, the product is not a part of $ \mathcal E $.

In the case that $ T_{j,z} \neq 0 $, then the same reasoning above applies to $ (TS)_{j,k} = T_{j,z} S_{z,k} $, where if $ S_{z,k} \neq 0 $ then the product is also non-zero, hence not a part of $ \mathcal E $.
